specs/ecdsap256/Spec.ECDSA.fst
@@ -472,8 +472,12 @@ let ecdsa_verification_agile alg publicKey r s mLen m =
       let u1D, _ = montgomery_ladder_spec u1 (pointAtInfinity, basePoint) in
       let u2D, _ = montgomery_ladder_spec u2 (pointAtInfinity, publicJacobian) in
 
-      let sumPoints = _point_add u1D u2D in
-      let pointNorm = _norm sumPoints in
+      let sumD = if  _norm u1D =  _norm u2D then
+       _point_double u1D
+      else 
+        _point_add u1D u2D in 
+      let pointNorm = _norm sumD in
+      
       let x, y, z = pointNorm in
       let x = x % prime_p256_order in 
       if Spec.P256.isPointAtInfinity pointNorm then false else x = r
